Linglib.lean
@@ -2816,7 +2816,7 @@ import Linglib.Syntax.Case.Order
 import Linglib.Syntax.Clause.Basic
 import Linglib.Syntax.Clause.Chaining
 import Linglib.Syntax.Clause.Complementation
-import Linglib.Syntax.Clause.Ctx
+import Linglib.Syntax.Clause.Context
 import Linglib.Syntax.Clause.Embedding
 import Linglib.Syntax.Clause.Frame
 import Linglib.Syntax.Comparative
